Continuing to work towards evaluation.

CircuitPath.dfy
@@ -10,47 +10,12 @@ module CircuitPath {
     import DG
     import Utils
 
-    predicate PathValid(lib: CLib, c: Circuit, p: seq<HPNP>)
-        requires CircuitValid(lib, c)
-    {
-        forall hpnp :: hpnp in p ==> HPNPValid(lib, c, hpnp)
-    }
-    
-    ghost predicate PathValidNoRepeats(lib: CLib, c: Circuit, p: seq<HPNP>)
-        requires CircuitValid(lib, c)
-    {
-        PathValid(lib, c, p) && Seq.HasNoDuplicates(p)
-    }
-
-    lemma PathLengthBound(lib: CLib, c: Circuit, p: seq<HPNP>)
-        requires CircuitValid(lib, c)
-        requires PathValidNoRepeats(lib, c, p)
-        ensures |p| <= CircuitBounds.HPNPBound(lib, c)
-    {
-        var bound := CircuitBounds.HPNPBound(lib, c);
-        forall hpnp: HPNP | hpnp in p
-            ensures HPNPToNat(hpnp) < bound
-        {
-            HPNPInBound(lib, c, hpnp);
-        }
-        var natted := Seq.Map(x => HPNPToNat(x), p);
-        forall a: HPNP, b: HPNP
-            ensures HPNPToNat(a) == HPNPToNat(b) ==> a == b
-        {
-            HPNPToNatInjective(a, b);
-        }
-        assert Functions.Injective(x => HPNPToNat(x));
-        SeqExt.MapConservesNoDuplicates(x => HPNPToNat(x), p);
-        assert Seq.HasNoDuplicates(natted);
-        Utils.SeqSize(natted, bound);
-        assert |natted| <= bound;
-    }
-
     predicate {:opaque} HPNPOtoIConnected(lib: CLib, c: Circuit, a: HPNP, b: HPNP)
         requires CircuitValid(lib, c)
         requires HPNPValidOutput(lib, c, a)
         requires HPNPValidInput(lib, c, b)
     {
+        HPNPValidHPValid(lib, c, a);
         var a_c := HierarchyPathCircuit(lib, c, a.hpn.hp);
         var maybe_a_nk := a_c.NodeKind(a.hpn.n);
         match maybe_a_nk
@@ -72,6 +37,7 @@ module CircuitPath {
                         false
             )
             case CHier(_) => (
+                reveal HPNPValidOutput();
                 var lower_c := NodeToSubcircuit(lib, a_c, a.hpn.n);
                 // It's an output port from a hier node.
                 // It only connects to the input into the corresponding Output node in that circuit.
@@ -95,10 +61,11 @@ module CircuitPath {
         requires HPNPValidInput(lib, c, a)
         requires HPNPValidOutput(lib, c, b)
     {
+        HPNPValidHPValid(lib, c, a);
         var a_c := HierarchyPathCircuit(lib, c, a.hpn.hp);
         var inp := NP(a.hpn.n, a.p);
         var onp := NP(b.hpn.n, b.p);
-        c.PortSource(inp) == Some(onp)
+        a_c.PortSource(inp) == Some(onp)
     }
 
     predicate {:opaque} HPNPConnected(lib: CLib, c: Circuit,  a: HPNP, b: HPNP)
@@ -140,6 +107,7 @@ module CircuitPath {
             assert nk.CHier?;
             HierarchyPathCircuitValid(lib, c, tail);
             assert CircuitValid(lib, tail_c);
+            reveal CircuitValid();
             assert CNodeKindValid(lib, tail_c, nk);
             assert tail_c.HierLevel > hier_c.HierLevel;
             HPLengthBound(lib, c, tail);
@@ -203,7 +171,7 @@ module CircuitPath {
         SeqNatToNat.ArbLenNatsToNatUnique(HPNPToSeqNat(a), HPNPToSeqNat(b));
     }
 
-    ghost function CtoG(lib: CLib, c: Circuit): (g: DG.Digraph<HPNP>)
+    function {:opaque} CtoG(lib: CLib, c: Circuit): (g: DG.Digraph<HPNP>)
         requires CircuitValid(lib, c)
     {
         DG.Digraph(
@@ -214,16 +182,29 @@ module CircuitPath {
         )
     }
 
+    function CtoGV(lib: CLib, c: Circuit): (g: DG.Digraph<HPNP>)
+        requires CircuitValid(lib, c)
+        ensures DG.DigraphValid(g)
+    {
+        CtoGValid(lib, c);
+        CtoG(lib, c)
+    }
+        
+
     lemma NoSelfConnections(lib: CLib, c: Circuit, n: HPNP)
         requires CircuitValid(lib, c)
         ensures !HPNPConnected(lib, c, n, n)
     {
         reveal HPNPConnected();
         if HPNPValid(lib, c, n) {
+            HPNPValidHPValid(lib, c, n);
             var hier_c := HierarchyPathCircuit(lib, c, n.hpn.hp);
             HierarchyPathCircuitValid(lib, c, n.hpn.hp);
+            reveal CircuitValid();
             assert CircuitNodeKindValid(lib, hier_c);
             if HPNPValidInput(lib, c, n) {
+                reveal HPNPValidInput();
+                reveal HPNPValidOutput();
                 assert !HPNPValidOutput(lib, c, n);
                 assert !HPNPConnected(lib, c, n, n);
             } else {
@@ -260,6 +241,7 @@ module CircuitPath {
         requires CircuitValid(lib, c)
         ensures DG.DigraphValid(CtoG(lib, c))
     {
+        reveal CtoG();
         var g := CtoG(lib, c);
         forall n: HPNP, m: HPNP
             ensures HPNPToNat(n) >= CircuitBounds.HPNPBound(lib, c) ==> !HPNPValid(lib, c, n)
@@ -309,18 +291,16 @@ module CircuitPath {
         requires HPNPValid(lib, c, hpnp)
         ensures HPNPToNat(hpnp) < CircuitBounds.HPNPBound(lib, c)
     {
-        CircuitBounds.HPNPElementsInBound(lib, c, hpnp);
         var hpnp_as_seq := HPNPToSeqNat(hpnp);
         var element_bound := CircuitBounds.HPNPElementBound(lib, c); 
         HPNPAsSeqNatInBound(lib, c, hpnp);
-
         var len := |hpnp_as_seq|;
-
         var bound := SeqNatToNat.ArbLenNatsToNatBound(c.HierLevel+2, element_bound);
         assert bound == CircuitBounds.HPNPBound(lib, c);
         assert forall n: nat :: n in hpnp_as_seq ==> n < element_bound;
         assert forall i: nat :: i < |hpnp_as_seq| ==> hpnp_as_seq[i] in hpnp_as_seq;
         assert forall i: nat :: i < |hpnp_as_seq| ==> hpnp_as_seq[i] < element_bound;
+        HPNPValidHPValid(lib, c, hpnp);
         HPLengthBound(lib, c, hpnp.hpn.hp);
         assert HPLength(hpnp.hpn.hp) <= c.HierLevel;
         assert |hpnp_as_seq| <= c.HierLevel + 2;
@@ -335,145 +315,68 @@ module CircuitPath {
         !DG.DigraphLoop(g)
     }
 
-    function {:vcs_split_on_every_assert} EvaluateINP(lib: CLib, c: Circuit, m: HPNP -> bool, inp: HPNP, seen_path: seq<HPNP>): bool
+    lemma NoLoopsMeansNotInPath(lib: CLib, c: Circuit, p: DG.Path<HPNP>, n: HPNP)
         requires CircuitValid(lib, c)
-        requires CircuitComplete(lib, c)
         requires CircuitNoLoops(lib, c)
-        requires HPNPValidInput(lib, c, inp)
-        decreases CircuitBounds.HPNPBound(lib, c) - |seen_path|, 1
+        requires PathValid(lib, c, p)
+        requires HPNPValid(lib, c, n)
+        requires |p.v| > 0 ==> HPNPConnected(lib, c, DG.PathEnd(p), n)
+        ensures n !in p.v
     {
-        var inp_c := HierarchyPathCircuit(lib, c, inp.hpn.hp);
-        HPCircuitComplete(lib, c, inp.hpn.hp);
-        assert CircuitComplete(lib, inp_c);
-        var inp_inp := NP(inp.hpn.n, inp.p);
-        var onp := inp_c.PortSource(inp_inp).value;
-        assert NPValidOutput(lib, inp_c, onp);
-        var new_seen_path := seen_path + [inp];
-        var hponp := HPNP(HPNode(inp.hpn.hp, onp.n), onp.p);
-        assert HPNPValidOutput(lib, c, hponp);
-        EvaluateONP(lib, c, m, hponp, new_seen_path)
+        var new_p := PathAppend(lib, c, p, n);
+        assert new_p == DG.Path(p.v + [n]);
+        assert PathValid(lib, c, new_p);
+        DG.NoLoopsMeansNoRepeats(CtoGV(lib, c));
+        assert DG.PathNoRepeats(new_p);
+        if n in p.v {
+            var index: nat :| index < |p.v| && p.v[index] == n;
+            assert new_p.v[index] == n;
+            assert new_p.v[|new_p.v|-1] == n;
+            assert !DG.PathNoRepeats(new_p);
+        }
     }
 
-    function {:vcs_split_on_every_assert} EvaluateONPCInput(lib: CLib, c: Circuit, isigs: HPNP -> bool, onp: HPNP,
-                               seen_path: seq<HPNP>): bool
+    function PathAppend(lib: CLib, c: Circuit, p: DG.Path<HPNP>, n: HPNP): (r: DG.Path<HPNP>)
+        // Just a PathAppend with more friendly requirements for a circuit.
         requires CircuitValid(lib, c)
-        requires CircuitComplete(lib, c)
-        requires CircuitNoLoops(lib, c)
-        requires HPNPValidOutput(lib, c, onp)
-        requires PathValidNoRepeats(lib, c, seen_path)
-        requires onp !in seen_path
-        requires 
-            var hp_c := HierarchyPathCircuit(lib, c, onp.hpn.hp);
-            var nk := hp_c.NodeKind(onp.hpn.n).value;
-            nk.CInput?
-        decreases CircuitBounds.HPNPBound(lib, c) - |seen_path|, 1
+        requires DG.PathValid(CtoGV(lib, c), p)
+        requires HPNPValid(lib, c, n)
+        requires (|p.v| > 0 ==> HPNPConnected(lib, c, DG.PathEnd(p), n))
+        ensures DG.PathValid(CtoGV(lib, c), r)
     {
-        var new_seen_path := seen_path + [onp];
-        NewSeenPathBound(lib, c, isigs, onp, seen_path);
-        if HPLength(onp.hpn.hp) == 0 then
-            // This is an input to the top level.
-            isigs(onp)
-        else
-            var (hier_n, parent_hp) := HPHeadTail(onp.hpn.hp);
-            assert HierarchyPathValid(lib, c, parent_hp);
-            // If it's an input inside a hier node, then it connects to
-            // the input port on the hier node on the next level up.
-            var inp := HPNP(HPNode(parent_hp, hier_n), onp.hpn.n as CPort);
-            var hier_c := HierarchyPathCircuit(lib, c, parent_hp);
-            HierarchyPathCircuitValid(lib, c, parent_hp);
-            var nk := hier_c.NodeKind(inp.hpn.n).value;
-            var cref := nk.CRef;
-            assert CircuitNodeKindValid(lib, hier_c);
-            var c := lib.Circuits[cref];
-            assert IsIPort(lib, nk, inp.p);
-            assert HPNPValidInput(lib, c, inp);
-            EvaluateINP(lib, c, isigs, inp, new_seen_path)
+        reveal CtoG();
+        DG.PathAppend(CtoGV(lib, c), p, n)
     }
 
-    function EvaluateONPCHier(
-            lib: CLib, c: Circuit, isigs: HPNP -> bool, onp: HPNP, seen_path: seq<HPNP>): bool
+    predicate PathValid(lib: CLib, c: Circuit, seen_path: DG.Path<HPNP>)
         requires CircuitValid(lib, c)
-        requires CircuitComplete(lib, c)
-        requires CircuitNoLoops(lib, c)
-        requires HPNPValidOutput(lib, c, onp)
-        requires PathValidNoRepeats(lib, c, seen_path)
-        requires onp !in seen_path
-        requires 
-            var hp_c := HierarchyPathCircuit(lib, c, onp.hpn.hp);
-            var nk := hp_c.NodeKind(onp.hpn.n).value;
-            nk.CHier?
-        decreases CircuitBounds.HPNPBound(lib, c) - |seen_path|, 1
     {
-        NewSeenPathBound(lib, c, isigs, onp, seen_path);
-        var hp_c := HierarchyPathCircuit(lib, c, onp.hpn.hp);
-        var new_seen_path := seen_path + [onp];
-        var lower_c := NodeToSubcircuit(lib, hp_c, onp.hpn.n);
-        // It's an output port from a hier node.
-        // It only connects to the input into the corresponding Output node in that circuit.
-
-        // The port number should reference an output port CNode inside the Circuit.
-        var maybe_level_nk := lower_c.NodeKind(onp.p as CNode);
-        assert maybe_level_nk.Some?;
-        assert maybe_level_nk.value.COutput?;
-        var new_hp := ExtendHierarchyPath(lib, c, onp.hpn.hp, onp.hpn.n);
-        EvaluateINP(lib, c, isigs, HPNP(HPNode(new_hp, onp.p as CNode), 0), new_seen_path)
+        DG.PathValid(CtoGV(lib, c), seen_path)
     }
 
-    function EvaluateONPCComb(
-            lib: CLib, c: Circuit, isigs: HPNP -> bool, onp: HPNP, seen_path: seq<HPNP>): bool
+    function NumberOfRemainingNodes(lib: CLib, c: Circuit, seen_path: DG.Path<HPNP>): nat
         requires CircuitValid(lib, c)
-        requires CircuitComplete(lib, c)
         requires CircuitNoLoops(lib, c)
-        requires HPNPValidOutput(lib, c, onp)
-        requires onp !in seen_path
-        requires 
-            var hp_c := HierarchyPathCircuit(lib, c, onp.hpn.hp);
-            var nk := hp_c.NodeKind(onp.hpn.n).value;
-            nk.CComb?
-        decreases CircuitBounds.HPNPBound(lib, c) - |seen_path|, 1
+        requires PathValid(lib, c, seen_path)
     {
-        true
+        DG.NoLoopsMeansNoRepeats(CtoGV(lib, c));
+        DG.NumberOfRemainingNodesPath(CtoGV(lib, c), seen_path)
     }
 
-    lemma NewSeenPathBound(lib: CLib, c: Circuit, isigns: HPNP -> bool, onp: HPNP,
-                           seen_path: seq<HPNP>)
+    lemma NumberOfRemainingNodesDecreases(lib: CLib, c: Circuit, seen_path: DG.Path<HPNP>, n: HPNP)
         requires CircuitValid(lib, c)
-        requires CircuitComplete(lib, c)
         requires CircuitNoLoops(lib, c)
-        requires PathValidNoRepeats(lib, c, seen_path)
-        requires HPNPValidOutput(lib, c, onp)
-        requires onp !in seen_path
-        ensures PathValidNoRepeats(lib, c, seen_path + [onp])
-        ensures |seen_path + [onp]| <= CircuitBounds.HPNPBound(lib, c)
+        requires PathValid(lib, c, seen_path)
+        requires HPNPValid(lib, c, n)
+        requires |seen_path.v| > 0 ==> HPNPConnected(lib, c, DG.PathEnd(seen_path), n)
+        ensures
+            var new_p := PathAppend(lib, c, seen_path, n);
+            NumberOfRemainingNodes(lib, c, new_p) <
+            NumberOfRemainingNodes(lib, c, seen_path)
     {
-        var hp_c := HierarchyPathCircuit(lib, c, onp.hpn.hp);
-        var nk := hp_c.NodeKind(onp.hpn.n).value;
-        var new_seen_path := seen_path + [onp];
-        reveal Seq.HasNoDuplicates();
-        assert |new_seen_path| > |seen_path|;
-        var bound := CircuitBounds.HPNPBound(lib, c);
-        PathLengthBound(lib, c, new_seen_path);
-        assert |new_seen_path| <= bound;
-        
+        DG.NoLoopsMeansNoRepeats(CtoGV(lib, c));
+        assert DG.PathNoRepeats(seen_path);
     }
 
-    function EvaluateONP(lib: CLib, c: Circuit, isigs: HPNP -> bool, onp: HPNP, seen_path: seq<HPNP>): bool
-        requires CircuitValid(lib, c)
-        requires CircuitComplete(lib, c)
-        requires CircuitNoLoops(lib, c)
-        requires PathValidNoRepeats(lib, c, seen_path)
-        requires HPNPValidOutput(lib, c, onp)
-        requires onp !in seen_path
-        decreases CircuitBounds.HPNPBound(lib, c) - |seen_path|, 2
-    {
-        var hp_c := HierarchyPathCircuit(lib, c, onp.hpn.hp);
-        var nk := hp_c.NodeKind(onp.hpn.n).value;
-        match nk
-        case CInput() => EvaluateONPCInput(lib, c, isigs, onp, seen_path)
-        case CHier(_) => EvaluateONPCHier(lib, c, isigs, onp, seen_path)
-        case CComb(_, _, _, _) => EvaluateONPCComb(lib, c, isigs, onp, seen_path)
-        case CSeq() => isigs(onp)
-        case CConst(v) => v
-    }
 
 }
