digraph.dfy
@@ -75,8 +75,7 @@ module DG {
     function PathAppend<Node>(g: Digraph, p: Path<Node>, n: Node): (r: Path<Node>)
         // Add a node onto a path.
         requires g.IsNode(n)
-        requires |p.v| > 0
-        requires g.IsConnected(p.v[|p.v|-1], n)
+        requires |p.v| > 0 ==> g.IsConnected(p.v[|p.v|-1], n)
         requires PathValid(g, p)
         ensures PathValid(g, r)
     {
@@ -154,6 +153,31 @@ module DG {
         // This path does not contain any repeated nodes.
     {
         forall i: nat, j: nat :: i < |p.v| && j < |p.v| && i != j ==> p.v[i] != p.v[j]
+    }
+
+    lemma NoLoopsMeansNoRepeats<Node(!new)>(g: Digraph<Node>)
+        requires !DigraphLoop(g)
+        ensures !exists p: Path<Node> :: PathValid(g, p) && !PathNoRepeats(p)
+    {
+        if exists p: Path<Node> :: PathValid(g, p) && !PathNoRepeats(p) {
+            var p : Path<Node> :| PathValid(g, p) && !PathNoRepeats(p);
+            assert PathValid(g, p);
+            var i: nat, j: nat :| (i < |p.v|) && (j < |p.v|) && (j > i) && (p.v[i] == p.v[j]);
+            var p_loop := PathSegment(p, i, j+1);
+            PathSegmentValid(g, p, i, j+1);
+            assert PathValid(g, p_loop);
+            assert PathLoop(p_loop);
+            reveal DigraphLoop();
+            assert DigraphLoop(g);
+            assert false;
+        }
+    }
+
+    lemma NoRepeatsIsHasNoDuplicates<Node>(p: Path<Node>)
+        requires PathNoRepeats(p)
+        ensures Seq.HasNoDuplicates(p.v)
+    {
+        reveal Seq.HasNoDuplicates();
     }
 
     predicate PathSimpleLoop<Node(==)>(p: Path<Node>)
@@ -388,6 +412,11 @@ module DG {
         Utils.BoundedSetSize(g.NodeBound as nat, nodes_as_nats);
     }
 
+    lemma MaxPathLength<Node>(g: Digraph, p: Path<Node>)
+        requires PathNoRepeats(p)
+    {
+    }
+
     function NumberOfRemainingNodes<Node>(g: Digraph, visited_nodes: set<Node>): nat
         // This is useful when we want to show that something that walks the
         // graph will terminate.
@@ -396,6 +425,23 @@ module DG {
     {
         NodeSetSize(g, visited_nodes);
         g.NodeBound - |visited_nodes|
+    }
+
+    function NumberOfRemainingNodesPath<Node(==)>(g: Digraph, p: Path<Node>): nat
+        // This is useful when we want to show that something that walks the
+        // graph will terminate.
+        requires DigraphValid(g)
+        requires PathValid(g, p)
+        requires PathNoRepeats(p)
+    {
+        NoRepeatsPathSetSize(p);
+        var s := PathSet(p);
+        assert forall x :: x in s ==> x in p.v;
+        reveal PathValid();
+        assert forall x :: x in p.v ==> g.IsNode(x);
+        NodeSetSize(g, s);
+        assert |p.v| <= g.NodeBound;
+        g.NodeBound - |p.v|
     }
 
     lemma NumberOfRemainingNodesDecreases<Node>(
@@ -411,9 +457,43 @@ module DG {
     {
     }
 
-    function PathSet<Node>(p: Path<Node>): (r: set<Node>)
+    function OneNodePath<Node>(g: Digraph, n: Node): (r: Path<Node>)
+        requires DigraphValid(g)
+        requires g.IsNode(n)
+        ensures PathValid(g, r)
     {
+        reveal PathValid();
+        Path([n])
+    }
+
+    lemma NumberOfRemainingNodesDecreasesPath<Node>(g: Digraph, p: Path<Node>, n: Node)
+        requires DigraphValid(g)
+        requires PathValid(g, p)
+        requires PathNoRepeats(p)
+        requires NodeValid(g, n)
+        requires g.IsNode(n)
+        requires |p.v| > 0 ==> g.IsConnected(PathEnd(p), n)
+        requires n !in p.v
+        ensures
+            var new_p := PathAppend(g, p, n);
+            NumberOfRemainingNodesPath(g, new_p) <
+            NumberOfRemainingNodesPath(g, p)
+    {
+    }
+
+    function PathSet<Node>(p: Path<Node>): (r: set<Node>)
+        ensures forall x :: x in r ==> x in p.v
+    {
+        reveal Seq.ToSet();
         Seq.ToSet(p.v)
+    }
+
+    lemma NoRepeatsPathSetSize<Node>(p: Path<Node>)
+        requires PathNoRepeats(p)
+        ensures |PathSet(p)| == |p.v|
+    {
+        NoRepeatsIsHasNoDuplicates(p);
+        Seq.LemmaCardinalityOfSetNoDuplicates(p.v);
     }
 
     lemma PathSetValid<Node>(g: Digraph, p: Path<Node>)
@@ -990,4 +1070,17 @@ module DG {
             assert DigraphLoop(g) || PathExists(g, m, n);
         }
     }
+
+    // We want to use this to be able to show for circuit that if we don't have loops then
+    // we can follow a path without worrying about infinite recursion.
+
+    // When we are following a path we have a variable that is the path we have been following.
+
+    // If a DG has no loops we can show:
+    // 1) The path has a maximum length.
+    // 2) If the next node is connected then the new path has no repeats and is longer.
+
+    //lemma NoReaPathLengthIsBound
+
+
 }
