CircuitStuff.dfy
@@ -1,0 +1,179 @@
+module CircuitStuff {
+
+    import opened Std.Wrappers
+    import Std.Collections.Seq
+    import opened Circuit
+    import opened CircuitPath
+    import DG
+
+    function {:opaque} INPtoONP(lib: CLib, c: Circuit, inp: HPNP): (onp: HPNP)
+        requires CircuitValid(lib, c)
+        requires CircuitComplete(lib, c)
+        requires HPNPValidInput(lib, c, inp)
+        ensures HPNPValidOutput(lib, c, onp)
+        ensures HPNPConnected(lib, c, inp, onp)
+    {
+        reveal HPNPConnected();
+        reveal HPNPItoOConnected();
+        reveal HPNPValidInput();
+        reveal HPNPValidOutput();
+        var inp_c := HierarchyPathCircuit(lib, c, inp.hpn.hp);
+        HPCircuitComplete(lib, c, inp.hpn.hp);
+        assert CircuitComplete(lib, inp_c);
+        var inp_inp := NP(inp.hpn.n, inp.p);
+        reveal CircuitComplete();
+        var onp_onp := inp_c.PortSource(inp_inp).value;
+        var onp := HPNP(HPNode(inp.hpn.hp, onp_onp.n), onp_onp.p);
+        reveal CircuitValid();
+        assert HPNPItoOConnected(lib, c, inp, onp);
+        onp
+    }
+
+    function {:opaque} ONPtoDeeperINP(lib: CLib, c: Circuit, onp: HPNP): (inp: HPNP)
+        requires CircuitValid(lib, c)
+        requires HPNPValidOutput(lib, c, onp)
+        requires HPNPtoNK(lib, c, onp).CHier?
+        ensures HPNPValidInput(lib, c, inp)
+        ensures HPNPConnected(lib, c, onp, inp)
+    {
+        HPNPValidHPValid(lib, c, onp);
+        var hp_c := HierarchyPathCircuit(lib, c, onp.hpn.hp);
+        HierarchyPathCircuitValid(lib, c, onp.hpn.hp);
+        var nk := HPNPtoNK(lib, c, onp);
+        assert CNodeKindValid(lib, hp_c, nk);
+        var lower_c := HPNPtoSubcircuit(lib, c, onp);
+        reveal HPNPValidOutput();
+        // It's an output port from a hier node.
+        // It only connects to the input into the corresponding Output node in that circuit.
+        // The port number should reference an output port CNode inside the Circuit.
+        var maybe_level_nk := lower_c.NodeKind(onp.p as CNode);
+        assert maybe_level_nk.Some?;
+        assert maybe_level_nk.value.COutput?;
+        var new_hp := ExtendHierarchyPath(lib, c, onp.hpn.hp, onp.hpn.n);
+        var inp := HPNP(HPNode(new_hp, onp.p as CNode), 0);
+        reveal HPNPConnected();
+        reveal HPNPOtoIConnected();
+        assert HPNPValidOutput(lib, c, onp);
+        reveal HPNPValidInput();
+        assert HPNPValidInput(lib, c, inp);
+        assert HPNPOtoIConnected(lib, c, onp, inp);
+        assert HPNPConnected(lib, c, onp, inp);
+        inp
+    }
+
+    function {:vcs_split_on_every_assert} EvaluateINP(
+            lib: CLib, c: Circuit, m: HPNP -> bool, p: DG.Path<HPNP>): bool
+        requires CircuitValid(lib, c)
+        requires CircuitComplete(lib, c)
+        requires CircuitNoLoops(lib, c)
+        requires |p.v| > 0
+        requires HPNPValidInput(lib, c, DG.PathEnd(p))
+        requires PathValid(lib, c, p)
+        decreases NumberOfRemainingNodes(lib, c, p), 1
+    {
+        var inp := DG.PathEnd(p);
+        var onp := INPtoONP(lib, c, inp);
+        assert HPNPValidOutput(lib, c, onp);
+        var new_p := PathAppend(lib, c, p, onp);
+        NoLoopsMeansNotInPath(lib, c, p, onp);
+        NumberOfRemainingNodesDecreases(lib, c, p, onp);
+        EvaluateONP(lib, c, m, new_p)
+    }
+
+    function {:vcs_split_on_every_assert} EvaluateONPCInput(
+            lib: CLib, c: Circuit, isigs: HPNP -> bool, p: DG.Path<HPNP>): bool
+        requires CircuitValid(lib, c)
+        requires CircuitComplete(lib, c)
+        requires CircuitNoLoops(lib, c)
+        requires |p.v| > 0
+        requires HPNPValidOutput(lib, c, DG.PathEnd(p))
+        requires PathValid(lib, c, p)
+        requires HPNPtoNK(lib, c, DG.PathEnd(p)).CInput?
+        decreases NumberOfRemainingNodes(lib, c, p), 1
+    {
+        var onp := DG.PathEnd(p);
+        if HPLength(onp.hpn.hp) == 0 then
+            // This is an input to the top level.
+            isigs(onp)
+        else
+            var (hier_n, parent_hp) := HPHeadTail(onp.hpn.hp);
+            HPNPValidHPValid(lib, c, onp);
+            assert HierarchyPathValid(lib, c, parent_hp);
+            // If it's an input inside a hier node, then it connects to
+            // the input port on the hier node on the next level up.
+            var inp := HPNP(HPNode(parent_hp, hier_n), onp.hpn.n as CPort);
+            var hier_c := HierarchyPathCircuit(lib, c, parent_hp);
+            HierarchyPathCircuitValid(lib, c, parent_hp);
+            var nk := hier_c.NodeKind(inp.hpn.n).value;
+            reveal CircuitValid();
+            reveal HPNPValidInput();
+            reveal HPNPValidOutput();
+            assert CircuitNodeKindValid(lib, hier_c);
+            assert IsIPort(lib, nk, inp.p);
+            assert HPNPValidInput(lib, c, inp);
+            var g := CtoG(lib, c);
+            DG.NoLoopsMeansNoRepeats(g);
+            reveal HPNPConnected();
+            reveal HPNPOtoIConnected();
+            assert HPNPConnected(lib, c, onp, inp);
+            var new_p := PathAppend(lib, c, p, inp);
+            NumberOfRemainingNodesDecreases(lib, c , p, inp);
+            EvaluateINP(lib, c, isigs, new_p)
+    }
+
+    function {:vcs_split_on_every_assert} EvaluateONPCHier(
+            lib: CLib, c: Circuit, isigs: HPNP -> bool, p: DG.Path<HPNP>): bool
+        requires CircuitValid(lib, c)
+        requires CircuitComplete(lib, c)
+        requires CircuitNoLoops(lib, c)
+        requires |p.v| > 0
+        requires HPNPValidOutput(lib, c, DG.PathEnd(p))
+        requires PathValid(lib, c, p)
+        requires HPNPtoNK(lib, c, DG.PathEnd(p)).CHier?
+        decreases NumberOfRemainingNodes(lib, c, p), 1
+    {
+        var onp := DG.PathEnd(p);
+        var inp := ONPtoDeeperINP(lib, c, onp);
+        var new_p := PathAppend(lib, c, p, inp);
+        NumberOfRemainingNodesDecreases(lib, c, p, inp);
+        EvaluateINP(lib, c, isigs, new_p)
+    }
+
+    function EvaluateONPCComb(
+            lib: CLib, c: Circuit, isigs: HPNP -> bool, p: DG.Path<HPNP>): bool
+        requires CircuitValid(lib, c)
+        requires CircuitComplete(lib, c)
+        requires CircuitNoLoops(lib, c)
+        requires PathValid(lib, c, p)
+        requires |p.v| > 0
+        requires HPNPValidOutput(lib, c, DG.PathEnd(p))
+        requires HPNPtoNK(lib, c, DG.PathEnd(p)).CComb?
+        decreases NumberOfRemainingNodes(lib, c, p), 1
+    {
+        true
+    }
+
+    function EvaluateONP(lib: CLib, c: Circuit, isigs: HPNP -> bool, p: DG.Path<HPNP>): bool
+        requires CircuitValid(lib, c)
+        requires CircuitComplete(lib, c)
+        requires CircuitNoLoops(lib, c)
+        requires PathValid(lib, c, p)
+        requires |p.v| > 0
+        requires HPNPValidOutput(lib, c, DG.PathEnd(p))
+        decreases NumberOfRemainingNodes(lib, c, p), 2
+    {
+        var onp := DG.PathEnd(p);
+        HPNPValidHPValid(lib, c, onp);
+        var hp_c := HierarchyPathCircuit(lib, c, onp.hpn.hp);
+        reveal HPNPValidOutput();
+        var nk := hp_c.NodeKind(onp.hpn.n).value;
+        match nk
+        case CInput() => EvaluateONPCInput(lib, c, isigs, p)
+        case CHier(_) => EvaluateONPCHier(lib, c, isigs, p)
+        case CComb(_, _, _, _) => EvaluateONPCComb(lib, c, isigs, p)
+        case CSeq() => isigs(onp)
+        case CConst(v) => v
+    }
+
+}
+
